some cleanup

specs/Spec.AESGCM.fst
@@ -14,7 +14,16 @@ let blocksize: size_nat = 16
 type key = lbytes keylen
 type bytes = s:seq UInt8.t{length s < pow2 32}
 
-(* TODO: rewrite with append *)
+val ghash_:
+  gmul_in_len:size_nat ->
+  gmul_in:lbytes gmul_in_len ->
+  tag_k:GF.key ->
+  k:GF.key ->
+  Tot GF.tag
+let ghash_ gmul_in_len gmul_in tag_k k =
+  let b0: GF.tag = AES.aes128_encrypt_block k (create blocksize (u8 0)) in
+  let h:lbytes blocksize = GF.gmac gmul_in_len gmul_in b0 tag_k in
+  h
 
 val ghash:
   text_len:size_nat ->
@@ -26,22 +35,18 @@ val ghash:
   Tot GF.tag
 let ghash text_len text aad_len aad tag_k k =
   (* gmul input: A || 0^v || C || 0^u || ceil(len(A))_64 || ceil(len(C))_64 *)
-  let aad_padding:size_nat = (16 - (aad_len % 16)) % 16 in
-  let text_padding:size_nat = (16 - (text_len % 16)) % 16 in
-  (* Build ghash input *)
-  let gmul_input_len = aad_len + aad_padding + text_len + text_padding + blocksize in
+  (* TODO: rewrite with concat *)
+  let aad_padding = (blocksize - (aad_len % blocksize)) % blocksize in
+  let text_padding = (blocksize - (text_len % blocksize)) % blocksize in
+  let gmul_input_len:size_nat = aad_len + aad_padding + text_len + text_padding + blocksize in
   let gmul_input = create gmul_input_len (u8 0) in
   let gmul_input = update_slice gmul_input 0 aad_len aad  in
-  (* padding is 0, so just skip those bytes *)
   let gmul_input = update_slice gmul_input (aad_len + aad_padding) (aad_len + aad_padding + text_len) text  in
-  (* padding is 0, so just skip those bytes *)
   let aad_len_bytes = nat_to_bytes_be 8 (aad_len * 8) in
   let gmul_input = update_slice gmul_input (aad_len + aad_padding + text_len + text_padding) (aad_len + aad_padding + text_len + text_padding + 8) aad_len_bytes  in
   let text_len_bytes = nat_to_bytes_be 8 (text_len * 8) in
-  let gmul_input = update_slice gmul_input (aad_len + aad_padding + text_len + text_padding + 8) (aad_len + aad_padding + text_len + text_padding + 16) text_len_bytes  in
-  let b0: GF.tag = AES.aes128_encrypt_block k (create 16 0uy) in
-  let h = GF.gmac gmul_input_len gmul_input b0 tag_k in
-  h
+  let gmul_input = update_slice gmul_input (aad_len + aad_padding + text_len + text_padding + 8) (aad_len + aad_padding + text_len + text_padding + blocksize) text_len_bytes  in
+  ghash_ gmul_input_len gmul_input tag_k k
 
 val gcm:
   k:key ->
@@ -53,7 +58,7 @@ val gcm:
   aad:lbytes aad_len ->
   Tot Spec.GF128.tag
 let gcm k n_len n m_len m aad_len aad =
-  let tag_key = AES.aes128_encrypt_bytes k n_len n 1 blocksize (create 16 0uy) in
+  let tag_key = AES.aes128_encrypt_bytes k n_len n 1 blocksize (create blocksize (u8 0)) in
   let mac = ghash m_len m aad_len aad tag_key k in
   mac
 
@@ -65,24 +70,20 @@ val aead_encrypt:
   m:lbytes len ->
   aad_len:size_nat{(len + aad_len) / blocksize <= max_size_t} ->
   aad:lbytes aad_len ->
-  Tot (lbytes (blocksize))
+  Tot (lbytes (len + blocksize))
 let aead_encrypt k n_len n len m aad_len aad =
-  let iv_len = if n_len = 12 then 12 else 16 in
+  let iv_len = if n_len = 12 then 12 else blocksize in
   let iv: lbytes iv_len = if n_len = 12 then n else (
-    (* TODO: rewrite ghash to re-use code. this is an ugly hack *)
     (* gmul input: IV || 0^(s+64) || ceil(len(IV))_64 *)
-    let n_padding:size_nat = (16 - (n_len % 16)) % 16 in
+    (* TODO: rewrite with concat *)
+    let n_padding:size_nat = (blocksize - (n_len % blocksize)) % blocksize in
     let n_padding = n_padding + 8 in
-    (* Build ghash input *)
     let gmul_input_len = n_len + n_padding + 8 in
     let gmul_input = create gmul_input_len (u8 0) in
     let gmul_input = update_slice gmul_input 0 n_len n  in
-    (* padding is 0, so just skip those bytes *)
     let n_len_bytes = nat_to_bytes_be 8 (n_len * 8) in
     let gmul_input = update_slice gmul_input (n_len + n_padding) (n_len + n_padding + 8) n_len_bytes  in
-    let b0: GF.tag = AES.aes128_encrypt_block k (create 16 0uy) in
-    let h:lbytes 16 = GF.gmac gmul_input_len gmul_input b0 (create 16 0uy) in
-    h
+    ghash_ gmul_input_len gmul_input (create blocksize (u8 0)) k
   ) in
   let c = AES.aes128_encrypt_bytes k iv_len iv 2 len m in
   let mac = gcm k iv_len iv len c aad_len aad in
