specs/Spec.AES.fst
@@ -23,11 +23,11 @@ open Spec.Lib.IntSeq
 
 (* Specialized imlplementation of GF(8) field *)
 
-(* let elem = uint8
+let elem = uint8
 let to_elem x = x
 let from_elem x = x
 let zero = u8 0
-let fadd (a:uint8) (b:uint8) : uint8 = a ^. b
+(* let fadd (a:uint8) (b:uint8) : uint8 = a ^. b *)
 let fmul (a:uint8) (b:uint8) : uint8 =
   let (p,a,b) =
     repeat 7 (fun (p,a,b) ->
@@ -64,13 +64,14 @@ let finv (a: uint8) =
 let sbox input =
   let s = finv input in
   let r: uint8 = logxor #U8 s ((s <<<. u32 1) ^. (s <<<. u32 2) ^. (s <<<. u32 3) ^. (s <<<. u32 4) ^. (u8 99)) in
-    r *)
+    r
 
 
 (* An S-Box circuit taken from Boyar-Peralta: http://cs-www.cs.yale.edu/homes/peralta/CircuitStuff/AESDEPTH16SIZE125 *)
 let (^~.) x y = logand #U8 (lognot #U8 (x ^. y)) (u8 1)
 
-let sbox input =
+(* TODO: re-enable. but this is so slow.... *)
+(* let sbox input =
   let u0 = input >>. u32 7 in
   let u1 = (input &. u8 64) >>. u32 6 in
   let u2 = (input &. u8 32) >>. u32 5 in
@@ -212,7 +213,7 @@ let sbox input =
   let s1 = t109 ^~. t140 in
     //uint8_t output = s0 ^. (s1 << 1) ^. (s2 << 2) ^. (s3 << 3) ^. (s4 << 4) ^. (s5 << 5) ^. (s6 << 6) ^. (s7 << 7);
   let output = s7 ^. (s6 <<. u32 1) ^. (s5 <<. u32 2) ^. (s4 <<. u32 3) ^. (s3 <<. u32 4) ^. (s2 <<. u32 5) ^. (s1 <<. u32 6) ^. (s0 <<. u32 7) in
-  output
+  output *)
 
 
 type block = lseq uint8 16
@@ -405,10 +406,10 @@ let aes_key_block (st:aes_state) : Tot block =
   let st = aes_init k n_len n in
   aes_key_block st *)
 
-let aes_key_block1 (k:block) (n:lseq uint8 12) : Tot block = 
+(* let aes_key_block1 (k:block) (n:lseq uint8 12) : Tot block =
   let st = aes_init k n in
   let st = aes_set_counter st 1 in
-  aes_key_block st
+  aes_key_block st *)
 
 let aes128_cipher =
   Spec.CTR.Cipher aes_state 16 max_size_t 16 aes_init aes_set_counter aes_key_block
